bindings.lean
@@ -1,0 +1,1063 @@
+import data.set
+
+import .syntax .freevars .vcgen
+
+lemma free_of_contains {P: prop} {σ: env} {x: var}: (⊢ σ : P) → x ∈ σ → x ∈ FV P :=
+  assume env_verified: ⊢ σ : P,
+  assume x_contained: x ∈ σ,
+  show x ∈ FV P, by begin
+    induction env_verified,
+    case env.vcgen.empty {
+      cases x_contained
+    },
+    case env.vcgen.tru σ' y Q _ _ ih { from
+      or.elim (env.contains.inv x_contained) (
+        assume : x = y,
+        have free_in_term x y, from this ▸ free_in_term.var x,
+        have free_in_term x (y ≡ value.true), from free_in_term.binop₁ this,
+        have free_in_prop x (y ≡ value.true), from free_in_prop.term this,
+        show x ∈ FV (Q ⋀ y ≡ value.true), from free_in_prop.and₂ this
+      ) (
+        assume : x ∈ σ',
+        have x ∈ FV Q, from ih this,
+        show x ∈ FV (Q ⋀ y ≡ value.true), from free_in_prop.and₁ this
+      )
+    },
+    case env.vcgen.fls σ' y Q _ _ ih { from
+      or.elim (env.contains.inv x_contained) (
+        assume : x = y,
+        have free_in_term x y, from this ▸ free_in_term.var x,
+        have free_in_term x (y ≡ value.false), from free_in_term.binop₁ this,
+        have free_in_prop x (y ≡ value.false), from free_in_prop.term this,
+        show x ∈ FV (Q ⋀ y ≡ value.false), from free_in_prop.and₂ this
+      ) (
+        assume : x ∈ σ',
+        have x ∈ FV Q, from ih this,
+        show x ∈ FV (Q ⋀ y ≡ value.false), from free_in_prop.and₁ this
+      )
+    },
+    case env.vcgen.num n σ' y Q _ _ ih { from
+      or.elim (env.contains.inv x_contained) (
+        assume : x = y,
+        have free_in_term x y, from this ▸ free_in_term.var x,
+        have free_in_term x (y ≡ value.num n), from free_in_term.binop₁ this,
+        have free_in_prop x (y ≡ value.num n), from free_in_prop.term this,
+        show x ∈ FV (Q ⋀ y ≡ value.num n), from free_in_prop.and₂ this
+      ) (
+        assume : x ∈ σ',
+        have x ∈ FV Q, from ih this,
+        show x ∈ FV (Q ⋀ y ≡ value.num n), from free_in_prop.and₁ this
+      )
+    },
+    case env.vcgen.func f σ₂ σ₁ g gx R S e H Q₁ Q₂ Q₃ _ _ _ _ _ _ _ fv_R fv_S e_verified _ ih₁ ih₂ { from
+      or.elim (env.contains.inv x_contained) (
+        assume : x = f,
+        have free_in_term x f, from this ▸ free_in_term.var x,
+        have free_in_term x (f ≡ value.func g gx R S e H σ₂), from free_in_term.binop₁ this,
+        have free_in_prop x (f ≡ value.func g gx R S e H σ₂), from free_in_prop.term this,
+        have x ∈ FV (prop.term (f ≡ value.func g gx R S e H σ₂) ⋀
+                     prop.subst_env (σ₂[g↦value.func g gx R S e H σ₂])
+                     (prop.func g gx R (Q₃ (term.app g gx) ⋀ S))), from free_in_prop.and₁ this,
+        show x ∈ FV (Q₁ ⋀ f ≡ value.func g gx R S e H σ₂ ⋀
+                     prop.subst_env (σ₂[g↦value.func g gx R S e H σ₂])
+                     (prop.func g gx R (Q₃ (term.app g gx) ⋀ S))), from free_in_prop.and₂ this
+      ) (
+        assume : x ∈ σ₁,
+        have x ∈ FV Q₁, from ih₁ this,
+        show x ∈ FV (Q₁ ⋀ f ≡ value.func g gx R S e H σ₂ ⋀
+                     prop.subst_env (σ₂[g↦value.func g gx R S e H σ₂])
+                     (prop.func g gx R (Q₃ (term.app g gx) ⋀ S))), from free_in_prop.and₁ this
+      )
+    }
+  end
+
+lemma exp.post_free {P: prop} {e: exp} {Q: propctx} {x: var}:
+       (P ⊢ e : Q) → ∀t, x ∈ FV (Q t) → x ∈ FV t ∨ x ∈ FV P :=
+  assume e_verified: P ⊢ e : Q,
+  begin
+    induction e_verified,
+    case exp.vcgen.tru P y e' Q y_not_in_P e'_verified ih { from
+      assume t: term,
+      assume x_free_in_Qt: x ∈ FV ((propctx.exis y ((y ≡ value.true) ⋀ Q)) t),
+      have x_neq_y: x ≠ y, from (free_in_propctx.exis.inv x_free_in_Qt).left,
+      have x_not_in_yv: x ∉ FV (y ≡ value.true), from (
+        assume : x ∈ FV (y ≡ value.true),
+        have free_in_term x y ∨ free_in_term x value.true, from free_in_term.binop.inv this,
+        or.elim this (
+          assume : free_in_term x y,
+          have x = y, from free_in_term.var.inv this,
+          show «false», from x_neq_y this
+        ) (
+          assume : free_in_term x value.true,
+          show «false», from free_in_term.value.inv this
+        )
+      ),
+      have x ∈ FV ((↑(y ≡ value.true) ⋀ Q) t), from (free_in_propctx.exis.inv x_free_in_Qt).right,
+      have x ∈ FV (propctx.term (y ≡ value.true) t) ∨ x ∈ FV (Q t), from free_in_propctx.and.inv this,
+      or.elim this (
+        assume : x ∈ FV (propctx.term (y ≡ value.true) t),
+        have x ∈ FV (((y ≡ value.true).to_termctx) t), from free_in_propctx.term.inv this,
+        have x ∈ FV (y ≡ value.true), from free_in_termctx.term.inv this,
+        show x ∈ FV t ∨ x ∈ FV P, from absurd this x_not_in_yv
+      ) (
+        assume : x ∈ FV (Q t),
+        have x ∈ FV t ∨ x ∈ FV (P ⋀ (y ≡ value.true)), from ih t this,
+        or.elim this (
+          assume : x ∈ FV t,
+          show x ∈ FV t ∨ x ∈ FV P, from or.inl this
+        ) (
+          assume : x ∈ FV (P ⋀ (y ≡ value.true)),
+          or.elim (free_in_prop.and.inv this) (
+            assume : x ∈ FV P,
+            show x ∈ FV t ∨ x ∈ FV P, from or.inr this
+          ) (
+            assume : x ∈ FV (prop.term (y ≡ value.true)),
+            have x ∈ FV (y ≡ value.true), from free_in_prop.term.inv this,
+            show x ∈ FV t ∨ x ∈ FV P, from absurd this x_not_in_yv
+          )
+        )
+      )
+    },
+    case exp.vcgen.fals P y e' Q y_not_in_P e'_verified ih { from
+      assume t: term,
+      assume x_free_in_Qt: x ∈ FV ((propctx.exis y ((y ≡ value.false) ⋀ Q)) t),
+      have x_neq_y: x ≠ y, from (free_in_propctx.exis.inv x_free_in_Qt).left,
+      have x_not_in_yv: x ∉ FV (y ≡ value.false), from (
+        assume : x ∈ FV (y ≡ value.false),
+        have free_in_term x y ∨ free_in_term x value.false, from free_in_term.binop.inv this,
+        or.elim this (
+          assume : free_in_term x y,
+          have x = y, from free_in_term.var.inv this,
+          show «false», from x_neq_y this
+        ) (
+          assume : free_in_term x value.false,
+          show «false», from free_in_term.value.inv this
+        )
+      ),
+      have x ∈ FV ((↑(y ≡ value.false) ⋀ Q) t), from (free_in_propctx.exis.inv x_free_in_Qt).right,
+      have x ∈ FV (propctx.term (y ≡ value.false) t) ∨ x ∈ FV (Q t), from free_in_propctx.and.inv this,
+      or.elim this (
+        assume : x ∈ FV (propctx.term (y ≡ value.false) t),
+        have x ∈ FV (((y ≡ value.false).to_termctx) t), from free_in_propctx.term.inv this,
+        have x ∈ FV (y ≡ value.false), from free_in_termctx.term.inv this,
+        show x ∈ FV t ∨ x ∈ FV P, from absurd this x_not_in_yv
+      ) (
+        assume : x ∈ FV (Q t),
+        have x ∈ FV t ∨ x ∈ FV (P ⋀ (y ≡ value.false)), from ih t this,
+        or.elim this (
+          assume : x ∈ FV t,
+          show x ∈ FV t ∨ x ∈ FV P, from or.inl this
+        ) (
+          assume : x ∈ FV (P ⋀ (y ≡ value.false)),
+          or.elim (free_in_prop.and.inv this) (
+            assume : x ∈ FV P,
+            show x ∈ FV t ∨ x ∈ FV P, from or.inr this
+          ) (
+            assume : x ∈ FV (prop.term (y ≡ value.false)),
+            have x ∈ FV (y ≡ value.false), from free_in_prop.term.inv this,
+            show x ∈ FV t ∨ x ∈ FV P, from absurd this x_not_in_yv
+          )
+        )
+      )
+    },
+    case exp.vcgen.num P y n e' Q y_not_in_P e'_verified ih { from
+      assume t: term,
+      assume x_free_in_Qt: x ∈ FV ((propctx.exis y ((y ≡ value.num n) ⋀ Q)) t),
+      have x_neq_y: x ≠ y, from (free_in_propctx.exis.inv x_free_in_Qt).left,
+      have x_not_in_yv: x ∉ FV (y ≡ value.num n), from (
+        assume : x ∈ FV (y ≡ value.num n),
+        have free_in_term x y ∨ free_in_term x (value.num n), from free_in_term.binop.inv this,
+        or.elim this (
+          assume : free_in_term x y,
+          have x = y, from free_in_term.var.inv this,
+          show «false», from x_neq_y this
+        ) (
+          assume : free_in_term x (value.num n),
+          show «false», from free_in_term.value.inv this
+        )
+      ),
+      have x ∈ FV ((↑(y ≡ value.num n) ⋀ Q) t), from (free_in_propctx.exis.inv x_free_in_Qt).right,
+      have x ∈ FV (propctx.term (y ≡ value.num n) t) ∨ x ∈ FV (Q t), from free_in_propctx.and.inv this,
+      or.elim this (
+        assume : x ∈ FV (propctx.term (y ≡ value.num n) t),
+        have x ∈ FV (((y ≡ value.num n).to_termctx) t), from free_in_propctx.term.inv this,
+        have x ∈ FV (y ≡ value.num n), from free_in_termctx.term.inv this,
+        show x ∈ FV t ∨ x ∈ FV P, from absurd this x_not_in_yv
+      ) (
+        assume : x ∈ FV (Q t),
+        have x ∈ FV t ∨ x ∈ FV (P ⋀ (y ≡ value.num n)), from ih t this,
+        or.elim this (
+          assume : x ∈ FV t,
+          show x ∈ FV t ∨ x ∈ FV P, from or.inl this
+        ) (
+          assume : x ∈ FV (P ⋀ (y ≡ value.num n)),
+          or.elim (free_in_prop.and.inv this) (
+            assume : x ∈ FV P,
+            show x ∈ FV t ∨ x ∈ FV P, from or.inr this
+          ) (
+            assume : x ∈ FV (prop.term (y ≡ value.num n)),
+            have x ∈ FV (y ≡ value.num n), from free_in_prop.term.inv this,
+            show x ∈ FV t ∨ x ∈ FV P, from absurd this x_not_in_yv
+          )
+        )
+      )
+    },
+    case exp.vcgen.func P f fx R S e₁ e₂ Q₁ Q₂ f_not_in_P _ _ _ fv_R fv_S _ _ func_vc ih₁ ih₂ { from
+      assume t: term,
+      assume x_free_in_Qt: x ∈ FV ((propctx.exis f ((prop.func f fx R (Q₁ (term.app f fx) ⋀ S)) ⋀ Q₂)) t),
+      have x_neq_f: x ≠ f, from (free_in_propctx.exis.inv x_free_in_Qt).left,
+      have x_not_in_non_rec_func: x ∈ FV (prop.func f fx R S) → x ∈ FV P, from (
+        assume : x ∈ FV (prop.func f fx R S),
+        have x ∈ FV (term.var f) ∨ (x ≠ fx ∧ (x ∈ FV R.to_prop ∨ x ∈ FV S.to_prop)),
+        from free_in_prop.func.inv this,
+        or.elim this (
+          assume : x ∈ FV (term.var f),
+          have x = f, from free_in_term.var.inv this,
+          show x ∈ FV P, from absurd this x_neq_f
+        ) (
+          assume : x ≠ fx ∧ (x ∈ FV R.to_prop ∨ x ∈ FV S.to_prop),
+          have x_neq_fx: x ≠ fx, from this.left,
+          or.elim this.right (
+            assume : x ∈ FV R.to_prop,
+            have x ∈ FV P ∪ {f, fx}, from set.mem_of_mem_of_subset this fv_R,
+            have x ∈ FV P ∨ x ∈ {f, fx}, from set.mem_or_mem_of_mem_union this,
+            or.elim this id (
+              assume : x ∈ {f, fx},
+              have (x = f) ∨ (x = fx), from set.two_elems_mem this,
+              or.elim this (
+                assume : x = f,
+                show x ∈ FV P, from absurd this x_neq_f
+              ) (
+                assume : x = fx,
+                show x ∈ FV P, from absurd this x_neq_fx
+              )
+            )
+          ) (
+            assume : x ∈ FV S.to_prop,
+            have x ∈ FV P ∪ {f, fx}, from set.mem_of_mem_of_subset this fv_S,
+            have x ∈ FV P ∨ x ∈ {f, fx}, from set.mem_or_mem_of_mem_union this,
+            or.elim this id (
+              assume : x ∈ {f, fx},
+              have (x = f) ∨ (x = fx), from set.two_elems_mem this,
+              or.elim this (
+                assume : x = f,
+                show x ∈ FV P, from absurd this x_neq_f
+              ) (
+                assume : x = fx,
+                show x ∈ FV P, from absurd this x_neq_fx
+              )
+            )
+          )
+        )
+      ),
+      have x_not_in_func: x ∈ FV (prop.func f fx R (Q₁ (term.app f fx) ⋀ S)) → x ∈ FV P, from (
+        assume : x ∈ FV (prop.func f fx R (Q₁ (term.app f fx) ⋀ S)),
+        have x ∈ FV (term.var f) ∨ (x ≠ fx ∧ (x ∈ FV R.to_prop ∨ x ∈ FV (Q₁ (term.app f fx) ⋀ S))),
+        from free_in_prop.func.inv this,
+        or.elim this (
+          assume : x ∈ FV (term.var f),
+          have x = f, from free_in_term.var.inv this,
+          show x ∈ FV P, from absurd this x_neq_f
+        ) (
+          assume : x ≠ fx ∧ (x ∈ FV R.to_prop ∨ x ∈ FV (Q₁ (term.app f fx) ⋀ S)),
+          have x_neq_fx: x ≠ fx, from this.left,
+          have x_not_in_R: x ∈ FV R.to_prop → x ∈ FV P, from (
+            assume : x ∈ FV R.to_prop,
+            have x ∈ FV P ∪ {f, fx}, from set.mem_of_mem_of_subset this fv_R,
+            have x ∈ FV P ∨ x ∈ {f, fx}, from set.mem_or_mem_of_mem_union this,
+            or.elim this id (
+              assume : x ∈ {f, fx},
+              have (x = f) ∨ (x = fx), from set.two_elems_mem this,
+              or.elim this (
+                assume : x = f,
+                show x ∈ FV P, from absurd this x_neq_f
+              ) (
+                assume : x = fx,
+                show x ∈ FV P, from absurd this x_neq_fx
+              )
+            )
+          ),
+          have x_not_in_S: x ∈ FV S.to_prop → x ∈ FV P, from (
+            assume : x ∈ FV S.to_prop,
+            have x ∈ FV P ∪ {f, fx}, from set.mem_of_mem_of_subset this fv_S,
+            have x ∈ FV P ∨ x ∈ {f, fx}, from set.mem_or_mem_of_mem_union this,
+            or.elim this id (
+              assume : x ∈ {f, fx},
+              have (x = f) ∨ (x = fx), from set.two_elems_mem this,
+              or.elim this (
+                assume : x = f,
+                show x ∈ FV P, from absurd this x_neq_f
+              ) (
+                assume : x = fx,
+                show x ∈ FV P, from absurd this x_neq_fx
+              )
+            )
+          ),
+          or.elim this.right x_not_in_R (
+            assume : x ∈ FV (Q₁ (term.app f fx) ⋀ S),
+            or.elim (free_in_prop.and.inv this) (
+              assume : x ∈ FV (Q₁ (term.app f fx)),
+              have x ∈ FV (term.app f fx) ∨ x ∈ FV (P ⋀ (spec.func f fx R S) ⋀ R), from ih₁ (term.app f fx) this,
+              or.elim this (
+                assume : x ∈ FV (term.app f fx),
+                have free_in_term x f ∨ free_in_term x fx, from free_in_term.app.inv this,
+                or.elim this (
+                  assume : free_in_term x f,
+                  have x = f, from free_in_term.var.inv this,
+                  show x ∈ FV P, from absurd this x_neq_f
+                ) (
+                  assume : free_in_term x fx,
+                  have x = fx, from free_in_term.var.inv this,
+                  show x ∈ FV P, from absurd this x_neq_fx
+                )
+              ) (
+                assume : x ∈ FV (P ⋀ (spec.func f fx R S) ⋀ R),
+                or.elim (free_in_prop.and.inv this) id (
+                  assume : x ∈ FV (prop.func f fx R S ⋀ R),
+                  or.elim (free_in_prop.and.inv this).symm x_not_in_R (
+                    assume : x ∈ FV (prop.func f fx R S),
+                    show x ∈ FV P, from x_not_in_non_rec_func this
+                  )
+                )
+              )
+            ) (
+              assume : x ∈ FV S.to_prop,
+              have x ∈ FV P ∪ {f, fx}, from set.mem_of_mem_of_subset this fv_S,
+              have x ∈ FV P ∨ x ∈ {f, fx}, from set.mem_or_mem_of_mem_union this,
+              or.elim this id (
+                assume : x ∈ {f, fx},
+                have (x = f) ∨ (x = fx), from set.two_elems_mem this,
+                or.elim this (
+                  assume : x = f,
+                  show x ∈ FV P, from absurd this x_neq_f
+                ) (
+                  assume : x = fx,
+                  show x ∈ FV P, from absurd this x_neq_fx
+                )
+              )
+            )
+          )
+        )
+      ),
+      have x ∈ FV ((propctx.and (prop.func f fx R (Q₁ (term.app f fx) ⋀ S)) Q₂) t),
+      from (free_in_propctx.exis.inv x_free_in_Qt).right,
+      have x ∈ FV ((prop.func f fx R (Q₁ (term.app f fx) ⋀ S)) t) ∨ x ∈ FV (Q₂ t),
+      from free_in_propctx.and.inv this,
+      or.elim this (
+        assume : x ∈ FV ((prop.func f fx R (Q₁ (term.app f fx) ⋀ S)) t),
+        have x ∈ FV (prop.func f fx R (Q₁ (term.app f fx) ⋀ S)), from free_in_propctx.prop.inv this,
+        show x ∈ FV t ∨ x ∈ FV P, from or.inr (x_not_in_func this)
+      ) (
+        assume : x ∈ FV (Q₂ t),
+        have x ∈ FV t ∨ x ∈ FV (P ⋀ prop.func f fx R (Q₁ (term.app f fx) ⋀ S)), from ih₂ t this,
+        or.elim this (
+          assume : x ∈ FV t,
+          show x ∈ FV t ∨ x ∈ FV P, from or.inl this
+        ) (
+          assume : x ∈ FV (P ⋀ prop.func f fx R (Q₁ (term.app f fx) ⋀ S)),
+          or.elim (free_in_prop.and.inv this) (
+            assume : x ∈ FV P,
+            show x ∈ FV t ∨ x ∈ FV P, from or.inr this
+          ) (
+            assume : x ∈ FV (prop.func f fx R (Q₁ (term.app f fx) ⋀ S)),
+            show x ∈ FV t ∨ x ∈ FV P, from or.inr (x_not_in_func this)
+          )
+        )
+      )
+    },
+    case exp.vcgen.unop op P e' x₁ y Q x_free_in_P y_not_in_P e'_verified vc_valid ih { from
+      assume t: term,
+      assume x_free_in_Qt: x ∈ FV ((propctx.exis y ((y ≡ term.unop op x₁) ⋀ Q)) t),
+      have x_neq_y: x ≠ y, from (free_in_propctx.exis.inv x_free_in_Qt).left,
+      have x_not_in_unop: x ∈ FV (y ≡ term.unop op x₁) → x ∈ FV P, from (
+        assume : x ∈ FV (y ≡ term.unop op x₁),
+        have free_in_term x y ∨ free_in_term x (term.unop op x₁), from free_in_term.binop.inv this,
+        or.elim this (
+          assume : free_in_term x y,
+          have x = y, from free_in_term.var.inv this,
+          show x ∈ FV P, from absurd this x_neq_y
+        ) (
+          assume : free_in_term x (term.unop op x₁),
+          have free_in_term x x₁, from free_in_term.unop.inv this,
+          have x = x₁, from free_in_term.var.inv this,
+          show x ∈ FV P, from this.symm ▸ x_free_in_P
+        )
+      ),
+      have x ∈ FV ((↑(y ≡ term.unop op x₁) ⋀ Q) t), from (free_in_propctx.exis.inv x_free_in_Qt).right,
+      have x ∈ FV (propctx.term (y ≡ term.unop op x₁) t) ∨ x ∈ FV (Q t), from free_in_propctx.and.inv this,
+      or.elim this (
+        assume : x ∈ FV (propctx.term (y ≡ term.unop op x₁) t),
+        have x ∈ FV (((y ≡ term.unop op x₁).to_termctx) t), from free_in_propctx.term.inv this,
+        have x ∈ FV (y ≡ term.unop op x₁), from free_in_termctx.term.inv this,
+        show x ∈ FV t ∨ x ∈ FV P, from or.inr (x_not_in_unop this)
+      ) (
+        assume : x ∈ FV (Q t),
+        have x ∈ FV t ∨ x ∈ FV (P ⋀ (y ≡ term.unop op x₁)), from ih t this,
+        or.elim this (
+          assume : x ∈ FV t,
+          show x ∈ FV t ∨ x ∈ FV P, from or.inl this
+        ) (
+          assume : x ∈ FV (P ⋀ (y ≡ term.unop op x₁)),
+          or.elim (free_in_prop.and.inv this) (
+            assume : x ∈ FV P,
+            show x ∈ FV t ∨ x ∈ FV P, from or.inr this
+          ) (
+            assume : x ∈ FV (prop.term (y ≡ term.unop op x₁)),
+            have x ∈ FV (y ≡ term.unop op x₁), from free_in_prop.term.inv this,
+            show x ∈ FV t ∨ x ∈ FV P, from or.inr (x_not_in_unop this)
+          )
+        )
+      )
+    },
+    case exp.vcgen.binop op P e' x₁ x₂ y Q x₁_free_in_P x₂_free_in_P y_not_in_P e'_verified vc_valid ih { from
+      assume t: term,
+      assume x_free_in_Qt: x ∈ FV ((propctx.exis y ((y ≡ term.binop op x₁ x₂) ⋀ Q)) t),
+      have x_neq_y: x ≠ y, from (free_in_propctx.exis.inv x_free_in_Qt).left,
+      have x_not_in_binop: x ∈ FV (y ≡ term.binop op x₁ x₂) → x ∈ FV P, from (
+        assume : x ∈ FV (y ≡ term.binop op x₁ x₂),
+        have free_in_term x y ∨ free_in_term x (term.binop op x₁ x₂), from free_in_term.binop.inv this,
+        or.elim this (
+          assume : free_in_term x y,
+          have x = y, from free_in_term.var.inv this,
+          show x ∈ FV P, from absurd this x_neq_y
+        ) (
+          assume : free_in_term x (term.binop op x₁ x₂),
+          have free_in_term x x₁ ∨ free_in_term x x₂, from free_in_term.binop.inv this,
+          or.elim this (
+            assume : free_in_term x x₁,
+            have x = x₁, from free_in_term.var.inv this,
+            show x ∈ FV P, from this.symm ▸ x₁_free_in_P
+          ) (
+            assume : free_in_term x x₂,
+            have x = x₂, from free_in_term.var.inv this,
+            show x ∈ FV P, from this.symm ▸ x₂_free_in_P
+          )
+        )
+      ),
+      have x ∈ FV ((↑(y ≡ term.binop op x₁ x₂) ⋀ Q) t), from (free_in_propctx.exis.inv x_free_in_Qt).right,
+      have x ∈ FV (propctx.term (y ≡ term.binop op x₁ x₂) t) ∨ x ∈ FV (Q t), from free_in_propctx.and.inv this,
+      or.elim this (
+        assume : x ∈ FV (propctx.term (y ≡ term.binop op x₁ x₂) t),
+        have x ∈ FV (((y ≡ term.binop op x₁ x₂).to_termctx) t), from free_in_propctx.term.inv this,
+        have x ∈ FV (y ≡ term.binop op x₁ x₂), from free_in_termctx.term.inv this,
+        show x ∈ FV t ∨ x ∈ FV P, from or.inr (x_not_in_binop this)
+      ) (
+        assume : x ∈ FV (Q t),
+        have x ∈ FV t ∨ x ∈ FV (P ⋀ (y ≡ term.binop op x₁ x₂)), from ih t this,
+        or.elim this (
+          assume : x ∈ FV t,
+          show x ∈ FV t ∨ x ∈ FV P, from or.inl this
+        ) (
+          assume : x ∈ FV (P ⋀ (y ≡ term.binop op x₁ x₂)),
+          or.elim (free_in_prop.and.inv this) (
+            assume : x ∈ FV P,
+            show x ∈ FV t ∨ x ∈ FV P, from or.inr this
+          ) (
+            assume : x ∈ FV (prop.term (y ≡ term.binop op x₁ x₂)),
+            have x ∈ FV (y ≡ term.binop op x₁ x₂), from free_in_prop.term.inv this,
+            show x ∈ FV t ∨ x ∈ FV P, from or.inr (x_not_in_binop this)
+          )
+        )
+      )
+    },
+    case exp.vcgen.app P y f e' x₁ Q f_free_in_P x₁_free_in_P y_not_in_P e'_verified vc_valid ih { from
+      assume t: term,
+      assume x_free_in_Qt: x ∈ FV ((propctx.exis y ((prop.call f x₁) ⋀
+                                                    (prop.post f x₁) ⋀
+                                                    (y ≡ term.app f x₁) ⋀
+                                                     Q)) t),
+      have x_neq_y: x ≠ y, from (free_in_propctx.exis.inv x_free_in_Qt).left,
+      have x_not_in_call: x ∈ FV (prop.call f x₁) → x ∈ FV P, from (
+        assume : x ∈ FV (prop.call f x₁),
+        or.elim (free_in_prop.call.inv this) (
+          assume : free_in_term x f,
+          have x = f, from free_in_term.var.inv this,
+          show x ∈ FV P, from this.symm ▸ f_free_in_P
+        ) (
+          assume : free_in_term x x₁,
+          have x = x₁, from free_in_term.var.inv this,
+          show x ∈ FV P, from this.symm ▸ x₁_free_in_P
+        )
+      ),
+      have x_not_in_post: x ∈ FV (prop.post f x₁) → x ∈ FV P, from (
+        assume : x ∈ FV (prop.post f x₁),
+        or.elim (free_in_prop.post.inv this) (
+          assume : free_in_term x f,
+          have x = f, from free_in_term.var.inv this,
+          show x ∈ FV P, from this.symm ▸ f_free_in_P
+        ) (
+          assume : free_in_term x x₁,
+          have x = x₁, from free_in_term.var.inv this,
+          show x ∈ FV P, from this.symm ▸ x₁_free_in_P
+        )
+      ),
+      have x_not_in_app: x ∈ FV (y ≡ term.app f x₁) → x ∈ FV P, from (
+        assume : x ∈ FV (y ≡ term.app f x₁),
+        have free_in_term x y ∨ free_in_term x (term.app f x₁), from free_in_term.binop.inv this,
+        or.elim this (
+          assume : free_in_term x y,
+          have x = y, from free_in_term.var.inv this,
+          show x ∈ FV P, from absurd this x_neq_y
+        ) (
+          assume : free_in_term x (term.app f x₁),
+          have free_in_term x f ∨ free_in_term x x₁, from free_in_term.app.inv this,
+          or.elim this (
+            assume : free_in_term x f,
+            have x = f, from free_in_term.var.inv this,
+            show x ∈ FV P, from this.symm ▸ f_free_in_P
+          ) (
+            assume : free_in_term x x₁,
+            have x = x₁, from free_in_term.var.inv this,
+            show x ∈ FV P, from this.symm ▸ x₁_free_in_P
+          )
+        )
+      ),
+      have x ∈ FV ((↑(prop.call ↑f ↑x₁) ⋀ ↑(prop.post ↑f ↑x₁) ⋀ ↑(↑y ≡ term.app ↑f ↑x₁) ⋀ Q) t),
+      from (free_in_propctx.exis.inv x_free_in_Qt).right,
+      have x ∈ FV (((prop.call f x₁):propctx) t) ∨ x ∈ FV ((↑(prop.post f x₁) ⋀ ↑(y ≡ term.app f x₁) ⋀ Q) t),
+      from free_in_propctx.and.inv this,
+      or.elim this (
+        assume : x ∈ FV (((prop.call f x₁):propctx) t),
+        have x ∈ FV (prop.call f x₁), from free_in_propctx.prop.inv this,
+        show x ∈ FV t ∨ x ∈ FV P, from or.inr (x_not_in_call this)
+      ) (
+        assume : x ∈ FV ((↑(prop.post f x₁) ⋀ ↑(y ≡ term.app f x₁) ⋀ Q) t),
+        have x ∈ FV (((prop.post f x₁):propctx) t) ∨ x ∈ FV ((↑(y ≡ term.app f x₁) ⋀ Q) t),
+        from free_in_propctx.and.inv this,
+        or.elim this (
+          assume : x ∈ FV (((prop.post f x₁):propctx) t),
+          have x ∈ FV (prop.post f x₁), from free_in_propctx.prop.inv this,
+          show x ∈ FV t ∨ x ∈ FV P, from or.inr (x_not_in_post this)
+        ) (
+          assume : x ∈ FV ((↑(y ≡ term.app f x₁) ⋀ Q) t),
+          have x ∈ FV ((↑(y ≡ term.app f x₁):propctx) t) ∨ x ∈ FV (Q t),
+          from free_in_propctx.and.inv this,
+          or.elim this (
+            assume : x ∈ FV (((y ≡ term.app f x₁):propctx) t),
+            have x ∈ FV ((y ≡ term.app f x₁):prop), from free_in_propctx.prop.inv this,
+            have x ∈ FV (y ≡ term.app f x₁), from free_in_prop.term.inv this,
+            show x ∈ FV t ∨ x ∈ FV P, from or.inr (x_not_in_app this)
+          ) (
+            assume : x ∈ FV (Q t),
+            have x ∈ FV t ∨ x ∈ FV (P ⋀ prop.call f x₁ ⋀ prop.post f x₁ ⋀ (y ≡ term.app f x₁)),
+            from ih t this,
+            or.elim this (
+              assume : x ∈ FV t,
+              show x ∈ FV t ∨ x ∈ FV P, from or.inl this
+            ) (
+              assume : x ∈ FV (P ⋀ prop.call f x₁ ⋀ prop.post f x₁ ⋀ (y ≡ term.app f x₁)),
+              or.elim (free_in_prop.and.inv this) (
+                assume : x ∈ FV P,
+                show x ∈ FV t ∨ x ∈ FV P, from or.inr this
+              ) (
+                assume : x ∈ FV (prop.call f x₁ ⋀ prop.post f x₁ ⋀ (y ≡ term.app f x₁)),
+                or.elim (free_in_prop.and.inv this) (
+                  assume : x ∈ FV (prop.call f x₁),
+                  show x ∈ FV t ∨ x ∈ FV P, from or.inr (x_not_in_call this)
+                ) (
+                  assume : x ∈ FV (prop.post f x₁ ⋀ (y ≡ term.app f x₁)),
+                  or.elim (free_in_prop.and.inv this) (
+                    assume : x ∈ FV (prop.post f x₁),
+                    show x ∈ FV t ∨ x ∈ FV P, from or.inr (x_not_in_post this)
+                  ) (
+                    assume : free_in_prop x (y ≡ term.app f x₁),
+                    have x ∈ FV (y ≡ term.app f x₁), from free_in_prop.term.inv this,
+                    show x ∈ FV t ∨ x ∈ FV P, from or.inr (x_not_in_app this)
+                  )
+                )
+              )
+            )
+          )
+        )
+      )
+    },
+    case exp.vcgen.ite P e₁ e₂ y Q₁ Q₂ y_free_in_P _ _ vc_valid ih₁ ih₂ { from
+      assume t: term,
+      assume x_free_in_Qt: x ∈ FV ((propctx.implies y Q₁ ⋀ propctx.implies (term.unop unop.not y) Q₂) t),
+      have x_not_in_y: free_in_prop x y → x ∈ FV P, from (
+        assume : free_in_prop x y,
+        have free_in_term x y, from free_in_prop.term.inv this,
+        have x = y, from free_in_term.var.inv this,
+        show x ∈ FV P, from this.symm ▸ y_free_in_P
+      ),
+      have x_not_in_yn: free_in_prop x (term.unop unop.not y) → x ∈ FV P, from (
+        assume : free_in_prop x (term.unop unop.not y),
+        have free_in_term x (term.unop unop.not y), from free_in_prop.term.inv this,
+        have free_in_term x y, from free_in_term.unop.inv this,
+        have x = y, from free_in_term.var.inv this,
+        show x ∈ FV P, from this.symm ▸ y_free_in_P
+      ),
+      or.elim (free_in_propctx.and.inv x_free_in_Qt) (
+        assume : x ∈ FV ((propctx.implies y Q₁) t),
+        or.elim (free_in_propctx.implies.inv this) (
+          assume : x ∈ FV ((prop.term y).to_propctx t),
+          have x ∈ FV (prop.term y), from free_in_propctx.prop.inv this,
+          show x ∈ FV t ∨ x ∈ FV P, from or.inr (x_not_in_y this)
+        ) (
+          assume : x ∈ FV (Q₁ t),
+          have x ∈ FV t ∨ x ∈ FV (P ⋀ y), from ih₁ t this,
+          or.elim this (
+            assume : x ∈ FV t,
+            show x ∈ FV t ∨ x ∈ FV P, from or.inl this
+          ) (
+            assume : x ∈ FV (P ⋀ y),
+            or.elim (free_in_prop.and.inv this) (
+              assume : x ∈ FV P,
+              show x ∈ FV t ∨ x ∈ FV P, from or.inr this
+            ) (
+              assume : free_in_prop x y,
+              have x ∈ FV P, from x_not_in_y this,
+              show x ∈ FV t ∨ x ∈ FV P, from or.inr this
+            )
+          )
+        )
+      ) (
+        assume : x ∈ FV ((propctx.implies (term.unop unop.not y) Q₂) t),
+        or.elim (free_in_propctx.implies.inv this) (
+          assume : x ∈ FV ((prop.term (term.unop unop.not y)).to_propctx t),
+          have x ∈ FV (prop.term (term.unop unop.not y)), from free_in_propctx.prop.inv this,
+          show x ∈ FV t ∨ x ∈ FV P, from or.inr (x_not_in_yn this)
+        ) (
+          assume : x ∈ FV (Q₂ t),
+          have x ∈ FV t ∨ x ∈ FV (P ⋀ (term.unop unop.not y)), from ih₂ t this,
+          or.elim this (
+            assume : x ∈ FV t,
+            show x ∈ FV t ∨ x ∈ FV P, from or.inl this
+          ) (
+            assume : x ∈ FV (P ⋀ (term.unop unop.not y)),
+            or.elim (free_in_prop.and.inv this) (
+              assume : x ∈ FV P,
+              show x ∈ FV t ∨ x ∈ FV P, from or.inr this
+            ) (
+              assume : free_in_prop x (term.unop unop.not y),
+              have x ∈ FV P, from x_not_in_yn this,
+              show x ∈ FV t ∨ x ∈ FV P, from or.inr this
+            )
+          )
+        )
+      )
+    },
+    case exp.vcgen.return P y y_free_in_P { from
+      assume t: term,
+      assume : x ∈ FV ((propctx.term (y ≣ •)) t),
+      have x ∈ FV ((y ≣ •) t), from free_in_propctx.term.inv this,
+      or.elim (free_in_termctx.binop.inv this) (
+        assume : x ∈ FV ((y:termctx) t),
+        have free_in_term x y, from free_in_termctx.term.inv this,
+        have x = y, from free_in_term.var.inv this,
+        have x ∈ FV P, from this.symm ▸ y_free_in_P,
+        show x ∈ FV t ∨ x ∈ FV P, from or.inr this
+      ) (
+        assume : x ∈ FV (• t),
+        have x ∈ FV t, from free_in_termctx.hole.inv this,
+        show x ∈ FV t ∨ x ∈ FV P, from or.inl this
+      )
+    }
+  end
+
+lemma contains_of_free_in_nonempty_env {σ: env} {x y: var} {v: value}:
+                                  (x ≠ y → y ∈ σ) → y ∈ (σ[x↦v]) :=
+  assume ih: x ≠ y → y ∈ σ,
+  if x_eq_y: x = y ∧ option.is_none (σ.apply y) then (
+    have h: σ[x↦v].apply x = (if x = x ∧ option.is_none (σ.apply x) then ↑v else σ.apply x), by unfold env.apply,
+    have (if x = x ∧ option.is_none (σ.apply x) then ↑v else σ.apply x) = ↑v, by simp [x_eq_y],
+    have σ[x↦v].apply x = ↑v, from eq.trans h this,
+    have σ[x↦v].apply y = some v, from x_eq_y.left ▸ this,
+    have ∃v', σ[x↦v] y = some v', from exists.intro v this,
+    show y ∈ (σ[x↦v]), from env.contains_apply_equiv.right.mp this
+  ) else (
+    have y ∈ σ, from (
+      have ¬(x = y) ∨ ¬(option.is_none (σ.apply y)), from not_and_distrib.mp x_eq_y,
+      this.elim (
+        assume : x ≠ y,
+        show y ∈ σ, from ih this        
+      ) ( 
+        assume : ¬(option.is_none (env.apply σ y)),
+        have ¬(option.is_none (σ y)), from this,
+        have option.is_some (σ y), from option.some_iff_not_none.mpr this,
+        have ∃v', σ y = some v', from option.is_some_iff_exists.mp this,
+        show y ∈ σ, from env.contains_apply_equiv.right.mp this
+      )
+    ),
+    let ⟨v', σ_has_y⟩ := (env.contains_apply_equiv.right.mpr this) in
+    have h: σ[x↦v].apply y = (if x = y ∧ option.is_none (σ.apply y) then ↑v else σ.apply y), by unfold env.apply,
+    have (if x = y ∧ option.is_none (σ.apply y) then ↑v else σ.apply y) = σ.apply y, by simp *,
+    have σ[x↦v].apply y = σ.apply y, from this ▸ h,
+    have σ[x↦v].apply y = some v', from eq.trans this σ_has_y,
+    have ∃v', σ[x↦v] y = some v', from exists.intro v' this,
+    show y ∈ (σ[x↦v]), from env.contains_apply_equiv.right.mp this
+  )
+
+lemma contains_of_free_eq_value {P: prop} {σ: env} {x y: var} {v: value}:
+  x ∈ FV (P ⋀ (y ≡ v)) → (x ∈ FV P → x ∈ σ) → x ∈ (σ[y↦v]) :=
+  assume x_free_in_P: x ∈ FV (P ⋀ (y ≡ v)),
+  assume ih : x ∈ FV P → x ∈ σ,
+  contains_of_free_in_nonempty_env (
+    assume x'_is_not_x: y ≠ x,
+    have free_in_prop x P ∨ free_in_prop x (y ≡ v), from free_in_prop.and.inv x_free_in_P,
+    or.elim this (
+      assume x_free_in_P: free_in_prop x P,
+      show x ∈ σ, from ih x_free_in_P
+    ) (
+      assume x_free_in_eq_v: free_in_prop x (y ≡ v),
+      show x ∈ σ, by begin
+        cases x_free_in_eq_v,
+        case free_in_prop.term x_free_in_eq {
+          cases x_free_in_eq,
+          case free_in_term.binop₁ free_in_y {
+            have y_is_x: (y = x), from (free_in_term.var.inv free_in_y).symm,
+            contradiction
+          },
+          case free_in_term.binop₂ free_in_v {
+            cases free_in_v
+          }
+        }
+      end
+    )
+  )
+
+lemma contains_of_free {P: prop} {σ: env} {x: var}: (⊢ σ : P) → free_in_prop x P → x ∈ σ :=
+  assume env_verified: ⊢ σ : P,
+  assume x_free_in_P: free_in_prop x P,
+  show x ∈ σ, by begin
+    induction env_verified,
+    case env.vcgen.empty { from
+      have free_in_term x value.true, from free_in_prop.term.inv x_free_in_P,
+      show x ∈ env.empty, from absurd this free_in_term.value.inv
+    },
+    case env.vcgen.tru σ' y Q _ _ ih {
+      show x ∈ (σ'[y↦value.true]), from contains_of_free_eq_value x_free_in_P ih
+    },
+    case env.vcgen.fls σ' y Q _ _ ih { from
+      show x ∈ (σ'[y↦value.false]), from contains_of_free_eq_value x_free_in_P ih
+    },
+    case env.vcgen.num n σ' y Q _ _ ih { from
+      show x ∈ (σ'[y↦value.num n]), from contains_of_free_eq_value x_free_in_P ih
+    },
+    case env.vcgen.func f σ₂ σ₁ g gx R S e H Q₁ Q₂ Q₃ _ _ _ _ _ _ _ fv_R fv_S e_verified _ ih₁ ih₂ { from
+      contains_of_free_in_nonempty_env (
+        assume : f ≠ x,
+        have x_neq_f: x ≠ f, from this.symm,
+        let vf := value.func g gx R S e H σ₂ in
+        have free_in_prop x Q₁
+           ∨ free_in_prop x ((f ≡ vf) ⋀ prop.subst_env (σ₂[g↦vf]) (prop.func g gx R (Q₃ (term.app g gx) ⋀ S))),
+        from free_in_prop.and.inv x_free_in_P,
+        or.elim this (
+          assume x_free_in_Q₁: free_in_prop x Q₁,
+          show x ∈ σ₁, from ih₁ x_free_in_Q₁
+        ) (
+          assume : free_in_prop x ((f ≡ vf) ⋀ prop.subst_env (σ₂[g↦vf]) (prop.func g gx R (Q₃ (term.app g gx) ⋀ S))),
+          or.elim (free_in_prop.and.inv this) (
+            assume x_free_in_eq_v: free_in_prop x (f ≡ vf),
+            show x ∈ σ₁, by begin
+              cases x_free_in_eq_v,
+              case free_in_prop.term x_free_in_eq {
+                cases x_free_in_eq,
+                case free_in_term.binop₁ free_in_f {
+                  have f_is_x: (f = x), from (free_in_term.var.inv free_in_f).symm,
+                  contradiction
+                },
+                case free_in_term.binop₂ free_in_vf {
+                  cases free_in_vf
+                }
+              }
+            end
+          ) (
+            assume x_free_in_sFunc: free_in_prop x (prop.subst_env (σ₂[g↦vf]) (prop.func g gx R (Q₃ (term.app g gx) ⋀ S))),
+            have x ≠ g ∧ free_in_prop x (prop.subst_env σ₂ (prop.func g gx R (Q₃ (term.app g gx) ⋀ S))),
+            from free_of_subst_env_prop x_free_in_sFunc,
+            have x_neq_g: x ≠ g, from this.left,
+            have x_free_in_sFunc': free_in_prop x (prop.subst_env σ₂ (prop.func g gx R (Q₃ (term.app g gx) ⋀ S))), from this.right,
+            have x_free_in_func: free_in_prop x (prop.func g gx R (Q₃ (term.app g gx) ⋀ S)),
+            from free_of_subst_env x_free_in_sFunc',
+            let forallp := (prop.implies R.to_prop (prop.pre g gx)
+                        ⋀ prop.implies (prop.post g gx) (Q₃ (term.app g gx) ⋀ S.to_prop)) in
+            have h: prop.func g gx R.to_prop (Q₃ (term.app g gx) ⋀ S.to_prop)
+                = (term.unop unop.isFunc g ⋀ prop.forallc gx g forallp),
+            by unfold prop.func,
+            have free_in_prop x (term.unop unop.isFunc g ⋀ prop.forallc gx g forallp), from h ▸ x_free_in_func,
+            have free_in_prop x (term.unop unop.isFunc g) ∨ free_in_prop x (prop.forallc gx g forallp),
+            from free_in_prop.and.inv this,
+            or.elim this (
+              assume : free_in_prop x (term.unop unop.isFunc g),
+              have free_in_term x (term.unop unop.isFunc g), from free_in_prop.term.inv this,
+              have free_in_term x g, from free_in_term.unop.inv this,
+              have x = g, from free_in_term.var.inv this,
+              show x ∈ σ₁, from absurd this x_neq_g
+            ) (
+              assume x_free_in_forallp: free_in_prop x (prop.forallc gx g forallp),
+              have x_neq_gx: x ≠ gx, from (free_in_prop.forallc.inv x_free_in_forallp).left,
+
+              have x_not_in_R: x ∉ FV R.to_prop, from (
+                assume : free_in_prop x R.to_prop,
+                have x ∈ FV Q₂ ∪ {g, gx}, from set.mem_of_mem_of_subset this fv_R,
+                have x ∈ FV Q₂ ∨ x ∈ {g, gx}, from set.mem_or_mem_of_mem_union this,
+                or.elim this (
+                  assume : x ∈ FV Q₂,
+                  have x ∈ σ₂, from ih₂ this,
+                  have ¬ free_in_prop x (prop.subst_env σ₂ (prop.func g gx R (Q₃ (term.app g gx) ⋀ S))),
+                  from prop.not_free_of_subst_env this,
+                  show «false», from this x_free_in_sFunc'
+                ) (
+                  assume : x ∈ {g, gx},
+                  have (x = g) ∨ (x = gx), from set.two_elems_mem this,
+                  or.elim this (
+                    assume : x = g,
+                    show «false», from x_neq_g this
+                  ) (
+                    assume : x = gx,
+                    show «false», from x_neq_gx this
+                  )
+                )
+              ),
+
+              have x_not_in_S: x ∉ FV S.to_prop, from (
+                assume : free_in_prop x S.to_prop,
+                have x ∈ FV Q₂ ∪ {g, gx}, from set.mem_of_mem_of_subset this fv_S,
+                have x ∈ FV Q₂ ∨ x ∈ {g, gx}, from set.mem_or_mem_of_mem_union this,
+                or.elim this (
+                  assume : x ∈ FV Q₂,
+                  have x ∈ σ₂, from ih₂ this,
+                  have ¬ free_in_prop x (prop.subst_env σ₂ (prop.func g gx R (Q₃ (term.app g gx) ⋀ S))),
+                  from prop.not_free_of_subst_env this,
+                  show «false», from this x_free_in_sFunc'
+                ) (
+                  assume : x ∈ {g, gx},
+                  have (x = g) ∨ (x = gx), from set.two_elems_mem this,
+                  or.elim this (
+                    assume : x = g,
+                    show «false», from x_neq_g this
+                  ) (
+                    assume : x = gx,
+                    show «false», from x_neq_gx this
+                  )
+                )
+              ),
+
+              have x_not_in_gfunc: x ∉ FV (prop.func g gx R S), from (
+                assume x_free_in_gfunc: x ∈ FV (prop.func g gx R S),
+                let forallp' := (prop.implies R.to_prop (prop.pre g gx)
+                              ⋀ prop.implies (prop.post g gx) S.to_prop) in
+                have h: prop.func g gx R.to_prop S.to_prop
+                    = (term.unop unop.isFunc g ⋀ prop.forallc gx g forallp'),
+                by unfold prop.func,
+                have free_in_prop x (term.unop unop.isFunc g ⋀ prop.forallc gx g forallp'), from h ▸ x_free_in_gfunc,
+                have free_in_prop x (term.unop unop.isFunc g) ∨ free_in_prop x (prop.forallc gx g forallp'),
+                from free_in_prop.and.inv this,
+                or.elim this (
+                  assume : free_in_prop x (term.unop unop.isFunc g),
+                  have free_in_term x (term.unop unop.isFunc g), from free_in_prop.term.inv this,
+                  have free_in_term x g, from free_in_term.unop.inv this,
+                  have x = g, from free_in_term.var.inv this,
+                  show «false», from x_neq_g this
+                ) (
+                  assume x_free_in_forallp': free_in_prop x (prop.forallc gx g forallp'),
+                  have x_neq_gx: x ≠ gx, from (free_in_prop.forallc.inv x_free_in_forallp').left,
+                  have free_in_term x g ∨ free_in_prop x forallp', from (free_in_prop.forallc.inv x_free_in_forallp').right,
+                  or.elim this (
+                    assume : free_in_term x g,
+                    have x = g, from free_in_term.var.inv this,
+                    show «false», from x_neq_g this
+                  ) (
+                    assume : free_in_prop x forallp',
+                    or.elim (free_in_prop.and.inv this) (
+                      assume : free_in_prop x (prop.implies R.to_prop (prop.pre g gx)),
+                      or.elim (free_in_prop.implies.inv this) x_not_in_R (
+                        assume : free_in_prop x (prop.pre g gx),
+                        have free_in_term x g ∨ free_in_term x gx, from free_in_prop.pre.inv this,
+                        or.elim this (
+                          assume : free_in_term x g,
+                          have x = g, from free_in_term.var.inv this,
+                          show «false», from x_neq_g this
+                        ) (
+                          assume : free_in_term x gx,
+                          have x = gx, from free_in_term.var.inv this,
+                          show «false», from x_neq_gx this
+                        )
+                      )
+                    ) (
+                      assume : free_in_prop x (prop.implies (prop.post g gx) S.to_prop),
+                      or.elim (free_in_prop.implies.inv this).symm x_not_in_S (
+                        assume : free_in_prop x (prop.post g gx),
+                        have free_in_term x g ∨ free_in_term x gx, from free_in_prop.post.inv this,
+                        or.elim this (
+                          assume : free_in_term x g,
+                          have x = g, from free_in_term.var.inv this,
+                          show «false», from x_neq_g this
+                        ) (
+                          assume : free_in_term x gx,
+                          have x = gx, from free_in_term.var.inv this,
+                          show «false», from x_neq_gx this
+                        )
+                      )
+                    )
+                  )
+                )
+              ),
+
+              have free_in_term x g ∨ free_in_prop x forallp, from (free_in_prop.forallc.inv x_free_in_forallp).right,
+              or.elim this (
+                assume : free_in_term x g,
+                have x = g, from free_in_term.var.inv this,
+                show x ∈ σ₁, from absurd this x_neq_g
+              ) (
+                assume : free_in_prop x forallp,
+                or.elim (free_in_prop.and.inv this) (
+                  assume : free_in_prop x (prop.implies R.to_prop (prop.pre g gx)),
+                  or.elim (free_in_prop.implies.inv this) (
+                    assume : x ∈ FV R.to_prop,
+                    show x ∈ σ₁, from absurd this x_not_in_R
+                  ) (
+                    assume : free_in_prop x (prop.pre g gx),
+                    have free_in_term x g ∨ free_in_term x gx, from free_in_prop.pre.inv this,
+                    or.elim this (
+                      assume : free_in_term x g,
+                      have x = g, from free_in_term.var.inv this,
+                      show x ∈ σ₁, from absurd this x_neq_g
+                    ) (
+                      assume : free_in_term x gx,
+                      have x = gx, from free_in_term.var.inv this,
+                      show x ∈ σ₁, from absurd this x_neq_gx
+                    )
+                  )
+                ) (
+                  assume : free_in_prop x (prop.implies (prop.post g gx) (Q₃ (term.app g gx) ⋀ S.to_prop)),
+                  or.elim (free_in_prop.implies.inv this) (
+                    assume : free_in_prop x (prop.post g gx),
+                    have free_in_term x g ∨ free_in_term x gx, from free_in_prop.post.inv this,
+                    or.elim this (
+                      assume : free_in_term x g,
+                      have x = g, from free_in_term.var.inv this,
+                      show x ∈ σ₁, from absurd this x_neq_g
+                    ) (
+                      assume : free_in_term x gx,
+                      have x = gx, from free_in_term.var.inv this,
+                      show x ∈ σ₁, from absurd this x_neq_gx
+                    )
+                  ) (
+                    assume : free_in_prop x (Q₃ (term.app g gx) ⋀ S.to_prop),
+                    have free_in_prop x (Q₃ (term.app g gx)) ∨ free_in_prop x S.to_prop, from free_in_prop.and.inv this,
+                    or.elim this.symm (
+                      assume : x ∈ FV S.to_prop,
+                      show x ∈ σ₁, from absurd this x_not_in_S
+                    ) (
+                      assume : free_in_prop x (Q₃ (term.app g gx)),
+                      have x ∈ FV (term.app g gx) ∨ x ∈ FV (↑H ⋀ Q₂ ⋀ (spec.func g gx R S) ⋀ R),
+                      from exp.post_free e_verified (term.app g gx) this,
+                      or.elim this (
+                        assume : x ∈ FV (term.app g gx),
+                        or.elim (free_in_term.app.inv this) (
+                          assume : free_in_term x g,
+                          have x = g, from free_in_term.var.inv this,
+                          show x ∈ σ₁, from absurd this x_neq_g
+                        ) (
+                        assume : free_in_term x gx,
+                        have x = gx, from free_in_term.var.inv this,
+                        show x ∈ σ₁, from absurd this x_neq_gx
+                        )
+                      ) (
+                        assume : x ∈ FV (↑H ⋀ Q₂ ⋀ (spec.func g gx R S) ⋀ R),
+                        or.elim (free_in_prop.and.inv this) (
+                          assume : x ∈ FV ↑H,
+                          have h: x ∈ FV ↑H, from this,
+                          have ↑H = calls_to_prop H, by refl,
+                          have x ∈ FV (calls_to_prop H), from this ▸ h,
+                          show x ∈ σ₁, from absurd this (call_history_closed H x)
+                        ) (
+                          assume : x ∈ FV (Q₂ ⋀ (spec.func g gx R S) ⋀ R),
+                          or.elim (free_in_prop.and.inv this) (
+                            assume : x ∈ FV Q₂,
+                            have x ∈ σ₂, from ih₂ this,
+                            have ¬ free_in_prop x (prop.subst_env σ₂ (prop.func g gx R (Q₃ (term.app g gx) ⋀ S))),
+                            from prop.not_free_of_subst_env this,
+                            show x ∈ σ₁, from absurd x_free_in_sFunc' this
+                          ) (
+                            assume : x ∈ FV (prop.func g gx R S ⋀ R),
+                            or.elim (free_in_prop.and.inv this) (
+                              assume : x ∈ FV (prop.func g gx R S),
+                              show x ∈ σ₁, from absurd this x_not_in_gfunc
+                            ) (
+                              assume : x ∈ FV R.to_prop,
+                              show x ∈ σ₁, from absurd this x_not_in_R
+                            )
+                          )
+                        )
+                      )
+                    )
+                  )
+                )
+              )
+            )
+          )
+        )
+      )
+   }
+ end
+
+lemma prop_func_closed {P: prop} {Q: propctx} {σ: env} {f fx: var} {R S: spec} {e: exp} {H: history}:
+  (H ⋀ P ⋀ spec.func f fx R S ⋀ R ⊢ e : Q) →
+  (⊢ (σ[f↦value.func f fx R S e H σ]) : (P
+       ⋀ (f ≡ value.func f fx R S e H σ)
+       ⋀ prop.subst_env (σ[f↦value.func f fx R S e H σ]) (prop.func f fx R (Q (term.app f fx) ⋀ S)))) →
+  ∀x, x ∉ FV (prop.subst_env (σ[f↦value.func f fx R S e H σ]) (prop.func f fx R (Q (term.app f fx) ⋀ S))) :=
+  assume e_verified: (H ⋀ P ⋀ spec.func f fx R S ⋀ R ⊢ e : Q),
+  assume env_verified: ⊢ (σ[f↦value.func f fx R S e H σ]) : (P
+       ⋀ (f ≡ value.func f fx R S e H σ)
+       ⋀ prop.subst_env (σ[f↦value.func f fx R S e H σ]) (prop.func f fx R (Q (term.app f fx) ⋀ S))),
+  assume x: var,
+  assume h: x ∈ FV (prop.subst_env (σ[f↦value.func f fx R S e H σ]) (prop.func f fx R (Q (term.app f fx) ⋀ S))),
+  have free_in_prop x (f ≡ value.func f fx R S e H σ
+       ⋀ prop.subst_env (σ[f↦value.func f fx R S e H σ]) (prop.func f fx R (Q (term.app f fx) ⋀ S))),
+  from free_in_prop.and₂ h,
+  have x ∈ FV (P
+       ⋀ (f ≡ value.func f fx R S e H σ)
+       ⋀ prop.subst_env (σ[f↦value.func f fx R S e H σ]) (prop.func f fx R (Q (term.app f fx) ⋀ S))),
+  from free_in_prop.and₂ this,
+  have x ∈ (σ[f↦value.func f fx R S e H σ]), from contains_of_free env_verified this,
+  have x ∉ FV (prop.subst_env (σ[f↦value.func f fx R S e H σ]) (prop.func f fx R (Q (term.app f fx) ⋀ S))),
+  from prop.not_free_of_subst_env this,
+  show «false», from this h
+
+lemma free_iff_contains {P: prop} {σ: env}: (⊢ σ : P) → (σ.dom = FV P) :=
+  assume σ_verified: ⊢ σ : P,
+  set.eq_of_subset_of_subset (
+    assume x: var,
+    assume : x ∈ σ.dom,
+    have x ∈ σ, from this,
+    show x ∈ FV P, from free_of_contains σ_verified this
+  ) (
+    assume x: var,
+    assume : x ∈ FV P,
+    have x ∈ σ, from contains_of_free σ_verified this,
+    show x ∈ σ.dom, from this
+  )
+
+lemma env.dom.inv {σ: env} {x: var} {v: value}: (σ[x↦v]).dom = (σ.dom ∪ set.insert x ∅) :=
+  set.eq_of_subset_of_subset (
+    assume y: var,
+    assume : y ∈ (σ[x↦v]).dom,
+    have y ∈ (σ[x↦v]), from this,
+    or.elim (env.contains.inv this) (
+      assume : y = x,
+      have y ∈ set.insert x ∅, from set.mem_singleton_of_eq this,
+      show y ∈ (σ.dom ∪ set.insert x ∅), from set.mem_union_right σ.dom this
+    ) (
+      assume : y ∈ σ,
+      have y ∈ σ.dom, from this,
+      show y ∈ (σ.dom ∪ set.insert x ∅), from set.mem_union_left (set.insert x ∅) this
+    )
+  ) (
+    assume y: var,
+    assume : y ∈ (σ.dom ∪ set.insert x ∅),
+    or.elim (set.mem_or_mem_of_mem_union this) (
+      assume : y ∈ σ.dom,
+      have y ∈ σ, from this,
+      have y ∈ (σ[x↦v]), from env.contains.rest this,
+      show y ∈ (σ[x↦v]).dom, from this
+    ) (
+      assume : y ∈ set.insert x ∅,
+      have y = x, from (set.mem_singleton_iff y x).mp this,
+      have y ∈ (σ[x↦v]), from this ▸ env.contains.same,
+      show y ∈ (σ[x↦v]).dom, from this
+    )
+  )
